move unnotransformed to paper_gni_example and cleanup

boogie_examples/all_exists/PCSat/paper_gni_example.bpl
@@ -30,93 +30,138 @@ procedure Unno (high: int, low: int) returns (r: int)
   r := x;
 }
 
+/* Hack to trigger instantiation. */
+function inst<a>(x: a) : bool { true }  
+
+procedure Unno_possNIalt (high: int, low: int, high': int, low': int) returns (x: int, x':int)
+          requires low == low';
+          ensures x == x'; 
+{ var b, b': int;   
+  var bsnap': int; // added by chk
+
+  if (high != 0 && high' != 0) { 
+     havoc x; 
+     assert (exists v:int :: x == v); // added by chk
+     havoc x'; assume x == x';  
+     if (x >= low || x' >= low') { /*skip*/ }
+     else { while (true) { /*skip*/ } }
+  }
+  else if (high != 0 && high' == 0) { 
+     havoc x;
+     if (x >= low) { /*skip*/ } 
+     else { while (true) { /*skip*/ } }
+      x' := low; 
+      assert inst(x - x');
+      assert (exists v:int :: {inst(v)} v == x - x'); // added by chk
+      havoc b'; assume b' == x - x'; 
+      while (b' != 0) 
+         invariant x >= x' && b' == x - x'; /* variant b' */
+      {  bsnap' := b'; // added by chk
+         x' := x' + 1; 
+         assert inst(x - x');
+         assert (exists v:int :: {inst(v)} v == x - x'); // added by chk
+         havoc b'; assume b' == x - x'; 
+         assert (0 <= b' && b' < bsnap'); // added by chk
+      }
+   }
+   else if (high == 0 && high' != 0) { 
+      x := low; 
+      havoc b;
+      while (b != 0)
+         invariant x >= low;
+      { x := x+1; havoc b; }
+      assert (exists v:int :: x == v); // added by chk
+      havoc x'; assume x == x'; 
+      if (x' >= low) { /*skip*/ }
+      else { while (true) { /*skip*/ } }
+    }
+    else { // high == 0 && high' == 0;
+       x := low; x' := low;
+       havoc b;
+       assert (exists v:int :: b == v); // added by chk
+       havoc b'; assume b == b'; 
+       while (b != 0 || b' != 0) 
+          invariant b == b' && x == x';
+       {  x := x+1; x' := x'+1;
+          havoc b;
+          assert (exists v:int :: b == v); // added by chk
+          havoc b'; assume b == b'; 
+       }
+    }
+}
+
+
+/* Alt version using trigger variable scheme,
+   and formatted compactly for use in slides.  */
+
 procedure Unno_possNI (high: int, low: int, high': int, low': int) returns (r: int, r':int)
           requires low == low';
           ensures r == r'; 
 { var x, x': int;
   var b, b': int;
   var bsnap': int;
+  var trigvar: int;
 
   if (high != 0 && high' != 0) { 
      havoc x; 
+     assert (exists v:int :: x == v); // inserted by chk
      havoc x'; assume x == x'; // HavocR x { Agree x };
      if (x >= low || x' >= low') { 
         call skip();
      }
      else { 
-//        ( while true do skip done | skip );
         while (true) { call skip(); } 
-        assert false; // added by user 
-//        ( skip | while true do variant { 0 } skip done );
         while (true) { call skip(); }
      }
-
-    assert x == x'; 
   }
-
   else if (high != 0 && high' == 0) { 
      havoc x;
      if (x >= low) { call skip(); } 
      else {  while (true) { call skip(); }  }
-   //      Assert { <| x >= low <] };
-      assert x >= low; 
       x' := low; 
-   //      HavocR b { [> b >] = [< x <] - [> x >] };
-      havoc b'; assume b' == x - x';
-   //      WhileR b <> 0 do
+      trigvar := x - x';
+      assert (exists v:int :: v == trigvar); // inserted by chk
+      havoc b'; assume b' == x - x'; // HavocR b
       while (b' != 0) 
-   //         invariant { [> b >= 0 |> }
          invariant b' >= 0;
-   //         invariant { [< x <] >= [> x >] }
          invariant x >= x';
-   //         invariant { [> b >] = [< x <] - [> x >] }
          invariant b' == x - x';
-   //         variant { [> b >] }
       {  
-         bsnap' := b'; // variant b'
+         bsnap' := b'; // variant b' inserted by chk
          x' := x' + 1; 
-   //        HavocR b { [> b >] = [< x <] - [> x >] }
-         havoc b'; assume b' == x - x';
-         assert 0 <= b' && b' < bsnap'; // variant decrease
+         trigvar := x - x';
+         assert (exists v:int :: v == trigvar); // inserted by chk
+         havoc b'; assume b' == x - x'; // HavocR b
+         assert (0 <= b' && b' < bsnap'); // variant decrease inserted by chk
       }
-
-    assert x == x'; 
    }
    else if (high == 0 && high' != 0) { 
-//       ( x := low; havoc b | skip );
       x := low;
       havoc b;
-//      WhileL b <> 0 do
       while (b != 0)
          invariant x >= low;
       { x := x+1; havoc b; }
-//      HavocR x { Agree x };
-      havoc x'; assume x == x'; 
+      assert (exists v:int :: x == v); // inserted by chk
+      havoc x'; assume x == x'; // HavocR x
       if (x' >= low) { call skip(); }
       else {
-         assert false; // added by user
          while (true) { call skip(); } 
       }
-    assert x == x'; 
     }
-    else { 
-       assert high == 0 && high' == 0;
+    else { // high == 0 && high' == 0;
        x := low; x' := low;
-//      ( havoc b | skip ); HavocR b { Agree b };
        havoc b;
-       havoc b'; assume b == b';
-//      While b <> 0 | b <> 0 . do
+       assert (exists v:int :: b == v); // inserted by chk
+       havoc b'; assume b == b'; // HavocR b
        while (b != 0 || b' != 0) 
           invariant b == b' && x == x';
        { 
           x := x+1; x' := x'+1;
           havoc b;
-//      HavocR b { Agree b };
-          havoc b'; assume b == b';
+          assert (exists v:int :: b == v); // inserted by chk
+          havoc b'; assume b == b'; // HavocR b 
        }
-    assert x == x'; 
-
     }
-    assert x == x'; 
     r := x; r' := x';
 }
+
